@base <http://data.europa.eu/s66#> .

@prefix : <http://www.semanticweb.org/owl/owlapi/turtle#> .
@prefix dc: <http://purl.org/dc/elements/1.1/> .
@prefix dcat: <http://www.w3.org/ns/dcat#> .
@prefix dcterms: <http://purl.org/dc/terms/> .
@prefix dg: <https://w3id.org/dingo#> .
@prefix eurio: <http://data.europa.eu/s66#> .
@prefix fabio: <http://purl.org/spar/fabio/> .
@prefix foaf: <http://xmlns.com/foaf/0.1/> .
@prefix frapo: <http://purl.org/cerif/frapo/> .
#@prefix oegp: <webode://droz.dia.fi.upm.es/Project+Ontology#> .
@prefix org: <http://www.w3.org/ns/org#> .
@prefix owl: <http://www.w3.org/2002/07/owl#> .
@prefix rdf: <http://www.w3.org/1999/02/22-rdf-syntax-ns#> .
@prefix rdfs: <http://www.w3.org/2000/01/rdf-schema#> .
@prefix schema: <http://schema.org/> .
@prefix skos: <http://www.w3.org/2004/02/skos/core#> .
@prefix vann: <http://purl.org/vocab/vann/> .
@prefix xsd: <http://www.w3.org/2001/XMLSchema#> .

<http://data.europa.eu/s66#> rdf:type owl:Ontology ;
                             owl:versionIRI <http://data.europa.eu/s66/v2.4#> ;
                             dc:creator "Publications Office of the European Commission"@en ;
                             dc:contributor "NTT Data";
                             dc:contributor "Cognizone";
                             dc:description "The EUropean Research Information Ontology (EURIO) conceptualises, formally encodes and makes available in an open, structured and machine-readable format data about research projects funded by the EU's framework programmes for research and innovation."@en ;
                             dc:publisher "Publications Office of the European Commission"@en ;
                             dc:title "EURIO: EUropean Research Information Ontology"@en ;

                             dcterms:license "https://creativecommons.org/licenses/by/4.0/"^^xsd:anyURI ;
                             dcterms:modified "2023-09-28"^^xsd:date ;
                             vann:preferredNamespacePrefix "eurio"^^xsd:string ;
                             rdfs:comment "CORDIS is the portal responsible for publishing the results of EU-funded research and innovation projects. EURIO (EUropean Research Information Ontology) is the conceptual data model developed by the Publications Office of the European Commission to represent and structure the CORDIS content in a semantic format improving its transparency, reusability and accessibility."@en ;
                             owl:versionInfo "v2.4"@en ;
                             dcat:distribution [ ] .

#################################################################
#    Annotation properties
#################################################################

###  http://purl.org/dc/elements/1.1/creator
dc:creator rdf:type owl:AnnotationProperty .


###  http://purl.org/dc/elements/1.1/description
dc:description rdf:type owl:AnnotationProperty .


###  http://purl.org/dc/elements/1.1/publisher
dc:publisher rdf:type owl:AnnotationProperty .


###  http://purl.org/dc/elements/1.1/title
dc:title rdf:type owl:AnnotationProperty .


###  http://purl.org/dc/terms/contributor
dcterms:contributor rdf:type owl:AnnotationProperty .


###  http://purl.org/dc/terms/license
dcterms:license rdf:type owl:AnnotationProperty .


###  http://purl.org/dc/terms/modified
dcterms:modified rdf:type owl:AnnotationProperty .


###  http://purl.org/vocab/vann/preferredNamespacePrefix
vann:preferredNamespacePrefix rdf:type owl:AnnotationProperty .


###  http://www.w3.org/2004/02/skos/core#broadMatch
skos:broadMatch rdf:type owl:AnnotationProperty .


###  http://www.w3.org/2004/02/skos/core#closeMatch
skos:closeMatch rdf:type owl:AnnotationProperty .


###  http://www.w3.org/2004/02/skos/core#definition
skos:definition rdf:type owl:AnnotationProperty .


###  http://www.w3.org/2004/02/skos/core#exactMatch
skos:exactMatch rdf:type owl:AnnotationProperty .


###  http://www.w3.org/2004/02/skos/core#note
skos:note rdf:type owl:AnnotationProperty .


###  http://www.w3.org/ns/dcat#accessURL
dcat:accessURL rdf:type owl:AnnotationProperty .


###  http://www.w3.org/ns/dcat#distribution
dcat:distribution rdf:type owl:AnnotationProperty .


###  http://www.w3.org/ns/dcat#downloadURL
dcat:downloadURL rdf:type owl:AnnotationProperty .


###  http://xmlns.com/foaf/0.1/mbox
foaf:mbox rdf:type owl:AnnotationProperty .


#################################################################
#    Datatypes
#################################################################

###  http://www.w3.org/2001/XMLSchema#date
xsd:date rdf:type rdfs:Datatype .


#################################################################
#    Object Properties
#################################################################

###  http://data.europa.eu/s66#disburses
eurio:disburses rdf:type owl:ObjectProperty ;
                owl:inverseOf eurio:isDisbursedBy ;
                rdfs:domain eurio:FundingAgency ;
                rdfs:range eurio:Grant ;
                rdfs:comment "Relates the funding agency to the grant(s) that it disburses."@en ;
                rdfs:isDefinedBy eurio: ;
                rdfs:label "disburses"@en .


###  http://data.europa.eu/s66#employs
eurio:employs rdf:type owl:ObjectProperty ;
              owl:inverseOf eurio:isEmployedBy ;
              rdfs:domain eurio:Organisation ;
              rdfs:range eurio:PersonRole ;
              rdfs:comment "Relates the organisation to the role representing a person that the organisation employs during a project in which both participate. "@en ;
              rdfs:isDefinedBy eurio: ;
              rdfs:label "employs"@en .


###  http://data.europa.eu/s66#funds
eurio:funds rdf:type owl:ObjectProperty ;
            owl:inverseOf eurio:isFundedBy ;
            rdfs:domain eurio:Grant ;
            rdfs:range eurio:Project ;
            rdfs:comment "Relates the grant with the project(s) that are completely or partially funded by it."@en ;
            rdfs:isDefinedBy eurio: ;
            rdfs:label "funds"@en .


###  http://data.europa.eu/s66#hasAcronym
eurio:hasAcronym rdf:type owl:ObjectProperty ;
                 owl:inverseOf eurio:isAcronymOf ;
                 rdfs:range eurio:Acronym ;
                 rdfs:comment "Relates an entity (e.g. project, grant, etc.) with its acronym(s). This includes acronyms representing the entity’s title as well as any additional acronyms extracted from other attributes of the entity."@en ;
                 rdfs:isDefinedBy eurio: ;
                 rdfs:label "has acronym"@en .


###  http://data.europa.eu/s66#hasAddress
eurio:hasAddress rdf:type owl:ObjectProperty ;
                 rdfs:domain eurio:Site ;
                 rdfs:range eurio:PostalAddress ;
                 rdfs:comment "Relates a physical location to its registered address."@en ;
                 rdfs:isDefinedBy eurio: ;
                 rdfs:label "has address"@en .


###  http://data.europa.eu/s66#hasAffiliatedOrganisation
#eurio:hasAffiliatedOrganisation rdf:type owl:ObjectProperty ;
#                                rdfs:range eurio:Organisation ;
#                                rdfs:comment "Relates the affiliated organisations of a publication."@en ;
#                                rdfs:isDefinedBy eurio: ;
#                                rdfs:label "has affiliated organisation"@en .


###  http://data.europa.eu/s66#hasAssociatedFundingScheme
eurio:hasAssociatedFundingScheme rdf:type owl:ObjectProperty ;
                                 rdfs:range eurio:FundingScheme ;
                                 rdfs:comment "Relates an entity other than funding scheme (e.g., result, etc.) with associated funding schemes."@en ;
                                 rdfs:isDefinedBy eurio: ;
                                 rdfs:label "has associated funding scheme"@en .


###  http://data.europa.eu/s66#hasBeneficiary
eurio:hasBeneficiary rdf:type owl:ObjectProperty ;
                     owl:inverseOf eurio:isBeneficiaryOf ;
                     rdfs:domain eurio:Grant ;
                     rdfs:range eurio:Role ;
                     rdfs:comment "Relates the grant to the organisation or person role(s) that are a beneficiary of the grant. "@en ;
                     rdfs:isDefinedBy eurio: ;
                     rdfs:label "has beneficiary"@en .


###  http://data.europa.eu/s66#hasContactDetails
eurio:hasContactDetails rdf:type owl:ObjectProperty ;
                        rdfs:range eurio:ContactPoint ;
                        rdfs:comment "Relates the role to the contact details of the entity taking the role (person or organisation) which are valid during the project of which the role forms a part."@en ;
                        rdfs:isDefinedBy eurio: ;
                        rdfs:label "has contact details"@en .


###  http://data.europa.eu/s66#hasCoordinates
eurio:hasCoordinates rdf:type owl:ObjectProperty ;
                     rdfs:domain eurio:Site ;
                     rdfs:range eurio:Coordinates ;
                     rdfs:comment "The geo-coordinates of a place"@en ;
                     rdfs:isDefinedBy eurio: ;
                     rdfs:label "has coordinates"@en .


###  http://data.europa.eu/s66#hasEUCountryCode
eurio:hasEUCountryCode rdf:type owl:ObjectProperty ;
                       rdfs:domain eurio:Country ;
                       rdfs:range skos:Concept ;
                       rdfs:comment "The country code of the location or address according to the EU country codes."@en ;
                       rdfs:isDefinedBy eurio: ;
                       rdfs:label "has EU country code"@en .


###  http://data.europa.eu/s66#hasEuroSciVocClassification
eurio:hasEuroSciVocClassification rdf:type owl:ObjectProperty ;
                                  rdfs:domain eurio:Project ;
                                  rdfs:range skos:Concept ;
                                  rdfs:comment "One or more values from the EuroSciVoc taxonomy that represent the main fields of science of the project."@en ;
                                  rdfs:isDefinedBy eurio: ;
                                  rdfs:label "has EuroSciVoc classification"@en .


####  http://data.europa.eu/s66#hasEvent
#eurio:hasEvent rdf:type owl:ObjectProperty ;
#               owl:inverseOf eurio:isEventOf ;
#               rdfs:domain eurio:Project ;
#               rdfs:range eurio:Event ;
#               rdfs:comment "Relates the project with its event(s)."@en ;
#               rdfs:isDefinedBy eurio: ;
#               rdfs:label "has event"@en .
#
#
####  http://data.europa.eu/s66#hasEventType
#eurio:hasEventType rdf:type owl:ObjectProperty ;
#                   rdfs:domain eurio:Event ;
#                   rdfs:range skos:Concept ;
#                   rdfs:comment "This is a controlled list of types of events."@en ;
#                   rdfs:isDefinedBy eurio: ;
#                   rdfs:label "has event type"@en .


###  http://data.europa.eu/s66#hasFundingAmount
eurio:hasFundingAmount rdf:type owl:ObjectProperty ;
                       rdfs:domain [ rdf:type owl:Class ;
                                     owl:unionOf ( eurio:FundingScheme
                                                   eurio:Grant
                                              )
                                ] ;
                       rdfs:range eurio:MonetaryAmount ;
                       rdfs:comment "Relates the grant or funding scheme to the amount of money available for funding."@en ;
                       rdfs:isDefinedBy eurio: ;
                       rdfs:label "has funding amount"@en .


###  http://data.europa.eu/s66#hasFundingScheme
eurio:hasFundingScheme rdf:type owl:ObjectProperty ;
                       owl:inverseOf eurio:hasGrant ;
                       rdfs:domain eurio:Grant ;
                       rdfs:range eurio:FundingScheme ;
                       rdfs:comment "Relates the grant to the funding scheme of which the grant forms a part."@en ;
                       rdfs:isDefinedBy eurio: ;
                       rdfs:label "has funding scheme"@en .


###  http://data.europa.eu/s66#hasFundingSchemeCall
eurio:hasFundingSchemeCall rdf:type owl:ObjectProperty ;
                           rdfs:subPropertyOf eurio:hasFundingScheme ;
                           rdfs:domain eurio:Grant ;
                           rdfs:range eurio:FundingScheme ;
                           rdfs:comment "Indicates the Call under which a project has been funded."@en ;
                           rdfs:isDefinedBy eurio: ;
                           rdfs:label "has funding scheme call"@en .


###  http://data.europa.eu/s66#hasFundingSchemeCategory
eurio:hasFundingSchemeCategory rdf:type owl:ObjectProperty ;
                               rdfs:domain eurio:FundingScheme ;
                               rdfs:range skos:Concept ;
                               rdfs:comment "A list of terms specifying the different categories / types of funding schemes."@en ;
                               rdfs:isDefinedBy eurio: ;
                               rdfs:label "has funding scheme category"@en .


###  http://data.europa.eu/s66#hasFundingSchemeProgramme
eurio:hasFundingSchemeProgramme rdf:type owl:ObjectProperty ;
                                rdfs:subPropertyOf eurio:hasFundingScheme ;
                                rdfs:domain eurio:Grant ;
                                rdfs:range eurio:FundingScheme ;
                                rdfs:comment "Indicates the legal basis under which a project has been funded."@en ;
                                rdfs:isDefinedBy eurio: ;
                                rdfs:label "has funding scheme programme"@en .


###  http://data.europa.eu/s66#hasFundingSchemeTopic
eurio:hasFundingSchemeTopic rdf:type owl:ObjectProperty ;
                            rdfs:subPropertyOf eurio:hasFundingScheme ;
                            rdfs:domain eurio:Grant ;
                            rdfs:range eurio:FundingScheme ;
                            rdfs:comment "Indicates the Topic under which a project has been funded."@en ;
                            rdfs:isDefinedBy eurio: ;
                            rdfs:label "has funding scheme topic"@en .


###  http://data.europa.eu/s66#hasFundingSchemeType
eurio:hasFundingSchemeType rdf:type owl:ObjectProperty ;
                           rdfs:subPropertyOf eurio:hasFundingScheme ;
                           rdfs:domain eurio:Grant ;
                           rdfs:range eurio:FundingScheme ;
                           rdfs:comment "Indicates the type of action under which a project has been funded."@en ;
                           rdfs:isDefinedBy eurio: ;
                           rdfs:label "has funding scheme type"@en .



###  http://data.europa.eu/s66#hasGeographicalLocation
eurio:hasGeographicalLocation rdf:type owl:ObjectProperty ;
                              rdfs:domain eurio:Site ;
                              rdfs:range eurio:AdministrativeArea ;
                              rdfs:comment "The basic containment relation between a place and one that contains it"@en ;
                              rdfs:isDefinedBy eurio: ;
                              rdfs:label "has geographical location"@en .


###  http://data.europa.eu/s66#hasGrant
eurio:hasGrant rdf:type owl:ObjectProperty ;
               rdfs:domain eurio:FundingScheme ;
               rdfs:range eurio:Grant ;
               rdfs:comment "Relates a funding scheme with the grants that form part of it. "@en ;
               rdfs:isDefinedBy eurio: ;
               rdfs:label "has grant"@en .


###  http://data.europa.eu/s66#hasISOCountryCode
eurio:hasISOCountryCode rdf:type owl:ObjectProperty ;
                        rdfs:domain eurio:Country ;
                        rdfs:range skos:Concept ;
                        rdfs:comment "The 2-digit ISO country code."@en ;
                        rdfs:isDefinedBy eurio: ;
                        rdfs:label "has ISO country code"@en .


###  http://data.europa.eu/s66#hasInvolvedParty
eurio:hasInvolvedParty rdf:type owl:ObjectProperty ;
                       owl:inverseOf eurio:isInvolvedIn ;
                       rdfs:domain eurio:Project ;
                       rdfs:range eurio:Role ;
                       rdfs:comment "Relates the Project to the roles that are involved in the project."@en ;
                       rdfs:isDefinedBy eurio: ;
                       rdfs:label "has involved party"@en .


###  http://data.europa.eu/s66#hasNUTS0code
eurio:hasNUTS0code rdf:type owl:ObjectProperty ;
                   rdfs:subPropertyOf eurio:hasNUTSCode ;
                   rdfs:domain eurio:AdministrativeArea ;
                   rdfs:range skos:Concept ;
                   rdfs:comment "A value representing the NUTS-0 code of the place or address."@en ;
                   rdfs:isDefinedBy eurio: ;
                   rdfs:label "has NUTS 0 code"@en .


###  http://data.europa.eu/s66#hasNUTS1code
eurio:hasNUTS1code rdf:type owl:ObjectProperty ;
                   rdfs:subPropertyOf eurio:hasNUTSCode ;
                   rdfs:domain eurio:AdministrativeArea ;
                   rdfs:range skos:Concept ;
                   rdfs:comment "A value representing the NUTS-1 code of the place or address."@en ;
                   rdfs:isDefinedBy eurio: ;
                   rdfs:label "has NUTS 1 code"@en .


###  http://data.europa.eu/s66#hasNUTS2code
eurio:hasNUTS2code rdf:type owl:ObjectProperty ;
                   rdfs:subPropertyOf eurio:hasNUTSCode ;
                   rdfs:domain eurio:AdministrativeArea ;
                   rdfs:range skos:Concept ;
                   rdfs:comment "A value representing the NUTS-2 code of the place or address."@en ;
                   rdfs:isDefinedBy eurio: ;
                   rdfs:label "has NUTS 2 code"@en .


###  http://data.europa.eu/s66#hasNUTS3code
eurio:hasNUTS3code rdf:type owl:ObjectProperty ;
                   rdfs:subPropertyOf eurio:hasNUTSCode ;
                   rdfs:domain eurio:AdministrativeArea ;
                   rdfs:range skos:Concept ;
                   rdfs:comment "A value representing the NUTS-3 code of the place or address."@en ;
                   rdfs:isDefinedBy eurio: ;
                   rdfs:label "has NUTS 3 code"@en .


###  http://data.europa.eu/s66#hasNUTSCode
eurio:hasNUTSCode rdf:type owl:ObjectProperty ;
                  rdfs:domain eurio:AdministrativeArea ;
                  rdfs:range skos:Concept ;
                  rdfs:comment "A value representing the NUTS code of the place or address."@en ;
                  rdfs:isDefinedBy eurio: ;
                  rdfs:label "has NUTS code"@en .


###  http://data.europa.eu/s66#hasNextFundingScheme
eurio:hasNextFundingScheme rdf:type owl:ObjectProperty ;
                           rdfs:domain eurio:FundingScheme ;
                           rdfs:range eurio:FundingScheme ;
                           rdfs:comment "Relates a funding scheme with the next funding scheme."@en ;
                           rdfs:isDefinedBy eurio: ;
                           rdfs:label "has next funding scheme"@en .


###  http://data.europa.eu/s66#hasPayment
eurio:hasPayment rdf:type owl:ObjectProperty ;
                 owl:inverseOf eurio:isPaymentOf ;
                 rdfs:domain eurio:Grant ;
                 rdfs:range eurio:GrantPayment ;
                 rdfs:comment "Relates the grant to its payment(s)."@en ;
                 rdfs:isDefinedBy eurio: ;
                 rdfs:label "has payment"@en .


###  http://data.europa.eu/s66#hasPaymentAmount
eurio:hasPaymentAmount rdf:type owl:ObjectProperty ;
                       rdfs:domain eurio:GrantPayment ;
                       rdfs:range eurio:MonetaryAmount ;
                       rdfs:comment "Relates the payment to the amount of money that was given to the beneficiary of the payment."@en ;
                       rdfs:isDefinedBy eurio: ;
                       rdfs:label "has payment amount"@en .


###  http://data.europa.eu/s66#hasPreviousFundingScheme
eurio:hasPreviousFundingScheme rdf:type owl:ObjectProperty ;
                               rdfs:domain eurio:FundingScheme ;
                               rdfs:range eurio:FundingScheme ;
                               rdfs:comment "Relates a funding scheme with the previous funding scheme."@en ;
                               rdfs:isDefinedBy eurio: ;
                               rdfs:label "has previous funding scheme"@en .


###  http://data.europa.eu/s66#hasProjectDivision
#eurio:hasProjectDivision rdf:type owl:ObjectProperty ;
#                         owl:inverseOf eurio:isDivisionOf ;
#                         rdfs:domain eurio:Project ;
#                         rdfs:range eurio:ProjectDivision ;
#                         rdfs:comment "Relates the project with its division(s)."@en ;
#                         rdfs:isDefinedBy eurio: ;
#                         rdfs:label "has project division"@en .


###  http://data.europa.eu/s66#hasRecipient
eurio:hasRecipient rdf:type owl:ObjectProperty ;
                   owl:inverseOf eurio:isRecipientOf ;
                   rdfs:domain eurio:GrantPayment ;
                   rdfs:range eurio:Role ;
                   rdfs:comment "Relates the grant payment to the organisation or person role(s) which have received the grant payment. Inverse property of isRecipientOf."@en ;
                   rdfs:isDefinedBy eurio: ;
                   rdfs:label "has recipient"@en .


###  http://data.europa.eu/s66#hasRelatedEvent
#eurio:hasRelatedEvent rdf:type owl:ObjectProperty ;
#                      rdfs:range eurio:Event ;
#                      rdfs:comment "Relates project-associated events."@en ;
#                      rdfs:isDefinedBy eurio: ;
#                      rdfs:label "has related event"@en .


###  http://data.europa.eu/s66#hasRelatedProject
eurio:hasRelatedProject rdf:type owl:ObjectProperty ,
                                 owl:SymmetricProperty ;
                        rdfs:domain eurio:Project ;
                        rdfs:range eurio:Project ;
                        rdfs:comment "Represents a generic non parent-child relation between two CORDIS projects."@en ;
                        rdfs:isDefinedBy eurio: ;
                        rdfs:label "has related project"@en .


###  http://data.europa.eu/s66#hasRelatedScheme
eurio:hasRelatedScheme rdf:type owl:ObjectProperty ,
                                owl:SymmetricProperty ;
                       rdfs:domain eurio:FundingScheme ;
                       rdfs:range eurio:FundingScheme ;
                       rdfs:comment "Represents a generic non parent-child relation between two funding schemes."@en ;
                       rdfs:isDefinedBy eurio: ;
                       rdfs:label "has related scheme"@en .


###  http://data.europa.eu/s66#hasResult
eurio:hasResult rdf:type owl:ObjectProperty ;
                owl:inverseOf eurio:isResultOf ;
                rdfs:domain [ rdf:type owl:Class ;
                              owl:unionOf ( eurio:Project
                                            #eurio:ProjectDivision
                                       )
                         ] ;
                rdfs:range eurio:Result ;
                rdfs:comment "Relates the project with its result(s)."@en ;
                rdfs:isDefinedBy eurio: ;
                rdfs:label "has result"@en .


###  http://data.europa.eu/s66#hasResultType
eurio:hasResultType rdf:type owl:ObjectProperty ;
                    rdfs:domain eurio:Result ;
                    rdfs:range skos:Concept ;
                    rdfs:comment "A list of terms specifying the types of results that can have a project."@en ;
                    rdfs:isDefinedBy eurio: ;
                    rdfs:label "has result type"@en .


###  http://data.europa.eu/s66#hasRole
eurio:hasRole rdf:type owl:ObjectProperty ;
              owl:inverseOf eurio:isRoleOf ;
              rdfs:domain [ rdf:type owl:Class ;
                            owl:unionOf ( eurio:Organisation
                                          eurio:Person
                                     )
                       ] ;
              rdfs:range eurio:Role ;
              rdfs:comment "Relates the person/organisation to the roles that the person/organisation takes."@en ;
              rdfs:isDefinedBy eurio: ;
              rdfs:label "has role"@en .


###  http://data.europa.eu/s66#hasSite
eurio:hasSite rdf:type owl:ObjectProperty ;
              rdfs:domain eurio:Organisation ;
              rdfs:range eurio:Site ;
              rdfs:comment "relates an organisation to its physical site"@en ;
              rdfs:isDefinedBy eurio: ;
              rdfs:label "has site"@en .


###  http://data.europa.eu/s66#hasSubDivision
#eurio:hasSubDivision rdf:type owl:ObjectProperty ;
#                     owl:inverseOf eurio:isSubDivisionOf ;
#                     rdfs:domain eurio:ProjectDivision ;
#                     rdfs:range eurio:ProjectDivision ;
#                     rdfs:comment "Relates a project division with its subdivisions."@en ;
#                     rdfs:isDefinedBy eurio: ;
#                     rdfs:label "has subdivision"@en .


###  http://data.europa.eu/s66#hasSubOrganisation
eurio:hasSubOrganisation rdf:type owl:ObjectProperty ;
                         owl:inverseOf eurio:isSubOrganisationOf ;
                         rdfs:domain eurio:Organisation ;
                         rdfs:range eurio:Organisation ;
                         rdfs:comment "Relates the organisation with another organisation which is a sub-part or child of it."@en ;
                         rdfs:isDefinedBy eurio: ;
                         rdfs:label "has sub-organisation"@en .


###  http://data.europa.eu/s66#hasSubScheme
eurio:hasSubScheme rdf:type owl:ObjectProperty ;
                   owl:inverseOf eurio:isSubSchemeOf ;
                   rdfs:domain eurio:FundingScheme ;
                   rdfs:range eurio:FundingScheme ;
                   rdfs:comment "Relates the funding scheme to its sub-schemes."@en ;
                   rdfs:isDefinedBy eurio: ;
                   rdfs:label "has subscheme"@en .


###  http://data.europa.eu/s66#hasTask
#eurio:hasTask rdf:type owl:ObjectProperty ;
#              owl:inverseOf eurio:isTaskOf ;
#              rdfs:domain eurio:WorkPackage ;
#              rdfs:range eurio:Task ;
#              rdfs:comment "Relates the work package to the task(s) that make up the package."@en ;
#              rdfs:isDefinedBy eurio: ;
#              rdfs:label "has task"@en .


###  http://data.europa.eu/s66#hasTotalCost
eurio:hasTotalCost rdf:type owl:ObjectProperty ;
                   rdfs:domain eurio:Project ;
                   rdfs:range eurio:MonetaryAmount ;
                   rdfs:comment "Relates the project with the amount of money expected, required, or given in payment for the project."@en ;
                   rdfs:isDefinedBy eurio: ;
                   rdfs:label "has total cost"@en .


###  http://data.europa.eu/s66#hasUnit
eurio:hasUnit rdf:type owl:ObjectProperty ;
              owl:inverseOf eurio:isUnitOf ;
              rdfs:domain eurio:Organisation ;
              rdfs:range eurio:OrganisationUnit ;
              rdfs:comment "Relates the organisation with a unit or department that forms part of the organisation."@en ;
              rdfs:isDefinedBy eurio: ;
              rdfs:label "has unit"@en .


###  http://data.europa.eu/s66#implements
eurio:implements rdf:type owl:ObjectProperty ;
                 owl:inverseOf eurio:isImplementedBy ;
                 rdfs:domain eurio:FundingAgency ;
                 rdfs:range eurio:FundingScheme ;
                 rdfs:comment "Relates a funding agency to the funding schemes that it implements and administers."@en ;
                 rdfs:isDefinedBy eurio: ;
                 rdfs:label "implements"@en .


###  http://data.europa.eu/s66#isAcronymOf
eurio:isAcronymOf rdf:type owl:ObjectProperty ;
                  rdfs:domain eurio:Acronym ;
                  rdfs:comment "Relates the acronym to the entity or entities to which it belongs."@en ;
                  rdfs:isDefinedBy eurio: ;
                  rdfs:label "is acronym of"@en .


###  http://data.europa.eu/s66#isBeneficiaryOf
eurio:isBeneficiaryOf rdf:type owl:ObjectProperty ;
                      rdfs:domain eurio:Role ;
                      rdfs:range eurio:Grant ;
                      rdfs:comment "Relates the role to the grant(s) of which the role is a beneficiary."@en ;
                      rdfs:isDefinedBy eurio: ;
                      rdfs:label "is beneficiary of"@en .


###  http://data.europa.eu/s66#isDisbursedBy
eurio:isDisbursedBy rdf:type owl:ObjectProperty ;
                    rdfs:domain eurio:Grant ;
                    rdfs:range eurio:FundingAgency ;
                    rdfs:comment "Relates the grant to the funding agency that disburses the grant."@en ;
                    rdfs:isDefinedBy eurio: ;
                    rdfs:label "is disbursed by"@en .


###  http://data.europa.eu/s66#isDivisionOf
#eurio:isDivisionOf rdf:type owl:ObjectProperty ;
#                   rdfs:domain eurio:ProjectDivision ;
#                   rdfs:range eurio:Project ;
#                   rdfs:comment "Relates the project division to the project of which it forms a part"@en ;
#                   rdfs:isDefinedBy eurio: ;
#                   rdfs:label "is division of"@en .


###  http://data.europa.eu/s66#isEmployedBy
eurio:isEmployedBy rdf:type owl:ObjectProperty ;
                   rdfs:domain eurio:PersonRole ;
                   rdfs:range eurio:Organisation ;
                   rdfs:comment "Relates the person role to the organisation in which the person holding the role is employed during the project."@en ;
                   rdfs:isDefinedBy eurio: ;
                   rdfs:label "is employed by"@en .


###  http://data.europa.eu/s66#isEventOf
#eurio:isEventOf rdf:type owl:ObjectProperty ;
#                rdfs:domain eurio:Event ;
#                rdfs:range eurio:Project ;
#                rdfs:comment "Relates the event to the project to which it belongs."@en ;
#                rdfs:isDefinedBy eurio: ;
#                rdfs:label "is event of"@en .


###  http://data.europa.eu/s66#isFundedBy
eurio:isFundedBy rdf:type owl:ObjectProperty ;
                 rdfs:domain eurio:Project ;
                 rdfs:range eurio:Grant ;
                 rdfs:comment "Relates the project with the grant(s) that completely or partially fund the project."@en ;
                 rdfs:isDefinedBy eurio: ;
                 rdfs:label "is funded by"@en .


###  http://data.europa.eu/s66#isHeldAt
#eurio:isHeldAt rdf:type owl:ObjectProperty ;
#               rdfs:domain eurio:Event ;
#               rdfs:range eurio:Site ;
#               rdfs:comment "The location where the event is happening."@en ;
#               rdfs:isDefinedBy eurio: ;
#               rdfs:label "is held at"@en .


###  http://data.europa.eu/s66#isImplementedBy
eurio:isImplementedBy rdf:type owl:ObjectProperty ;
                      rdfs:domain eurio:FundingScheme ;
                      rdfs:range eurio:FundingAgency ;
                      rdfs:comment "Relates the funding scheme with the funding agency that implements and administers the scheme."@en ;
                      rdfs:isDefinedBy eurio: ;
                      rdfs:label "is implemented by"@en .


###  http://data.europa.eu/s66#isInvolvedIn
eurio:isInvolvedIn rdf:type owl:ObjectProperty ;
                   rdfs:domain eurio:Role ;
                   rdfs:range eurio:Project ;
                   rdfs:comment "Relates the role to the Project in which it is involved."@en ;
                   rdfs:isDefinedBy eurio: ;
                   rdfs:label "is involved in"@en .


###  http://data.europa.eu/s66#isPaymentOf
eurio:isPaymentOf rdf:type owl:ObjectProperty ;
                  rdfs:domain eurio:GrantPayment ;
                  rdfs:range eurio:Grant ;
                  rdfs:comment "Relates a payment to the grant of which it is a part."@en ;
                  rdfs:isDefinedBy eurio: ;
                  rdfs:label "is payment of"@en .


###  http://data.europa.eu/s66#isRecipientOf
eurio:isRecipientOf rdf:type owl:ObjectProperty ;
                    rdfs:domain eurio:Role ;
                    rdfs:range eurio:GrantPayment ;
                    rdfs:comment "Relates the organisation or person role with the grant payment(s) which they have received. Inverse property of hasRecipient."@en ;
                    rdfs:isDefinedBy eurio: ;
                    rdfs:label "is recipient of"@en .


###  http://data.europa.eu/s66#isResultOf
eurio:isResultOf rdf:type owl:ObjectProperty ;
                 rdfs:domain eurio:Result ;
                 rdfs:range [ rdf:type owl:Class ;
                              owl:unionOf ( eurio:Project
                                            #eurio:ProjectDivision
                                       )
                          ] ;
                 rdfs:comment "Relates the results with the Project(s) involved."@en ;
                 rdfs:isDefinedBy eurio: ;
                 rdfs:label "is result of"@en .


###  http://data.europa.eu/s66#isRoleOf
eurio:isRoleOf rdf:type owl:ObjectProperty ;
               rdfs:domain eurio:Role ;
               rdfs:range [ rdf:type owl:Class ;
                            owl:unionOf ( eurio:Organisation
                                          eurio:Person
                                     )
                        ] ;
               rdfs:comment "Relates the person/organisation role to the person/organisation which assumes the role."@en ;
               rdfs:isDefinedBy eurio: ;
               rdfs:label "is role of"@en .


###  http://data.europa.eu/s66#isSiteOf
eurio:isSiteOf rdf:type owl:ObjectProperty ;
               rdfs:domain eurio:Site ;
               rdfs:range eurio:Organisation ;
               rdfs:comment "Indicates an entity which has presence at the given site"@en ;
               rdfs:isDefinedBy eurio: ;
               rdfs:label "is site of"@en .


###  http://data.europa.eu/s66#isSubDivisionOf
#eurio:isSubDivisionOf rdf:type owl:ObjectProperty ;
#                      rdfs:domain eurio:ProjectDivision ;
#                      rdfs:range eurio:ProjectDivision ;
#                      rdfs:comment "Relates a project division with its parent division."@en ;
#                      rdfs:isDefinedBy eurio: ;
#                      rdfs:label "is subdivision of"@en .


###  http://data.europa.eu/s66#isSubOrganisationOf
eurio:isSubOrganisationOf rdf:type owl:ObjectProperty ;
                          rdfs:domain eurio:Organisation ;
                          rdfs:range eurio:Organisation ;
                          rdfs:comment "Relates the organisation with another organisation of which it is a sub-part."@en ;
                          rdfs:isDefinedBy eurio: ;
                          rdfs:label "is sub-organisation of"@en .


###  http://data.europa.eu/s66#isSubSchemeOf
eurio:isSubSchemeOf rdf:type owl:ObjectProperty ;
                    rdfs:domain eurio:FundingScheme ;
                    rdfs:range eurio:FundingScheme ;
                    rdfs:comment "Relates the funding scheme to its parent scheme of which this funding scheme forms a part. "@en ;
                    rdfs:isDefinedBy eurio: ;
                    rdfs:label "is subscheme of"@en .


###  http://data.europa.eu/s66#isTaskOf
#eurio:isTaskOf rdf:type owl:ObjectProperty ;
#               rdfs:domain eurio:Task ;
#               rdfs:range eurio:WorkPackage ;
#               rdfs:comment "Relates the task to the work package of which it is a part."@en ;
#               rdfs:isDefinedBy eurio: ;
#               rdfs:label "is task of"@en .


###  http://data.europa.eu/s66#isUnitOf
eurio:isUnitOf rdf:type owl:ObjectProperty ;
               rdfs:domain eurio:OrganisationUnit ;
               rdfs:range eurio:Organisation ;
               rdfs:comment "Relates the unit to the organisation of which the unit forms a part. "@en ;
               rdfs:isDefinedBy eurio: ;
               rdfs:label "is unit of"@en .


###  http://data.europa.eu/s66#refersTo
eurio:refersTo rdf:type owl:ObjectProperty ;
               rdfs:domain eurio:Acronym ;
               rdfs:comment "The entity to which this acronym refers. This can either be an entity inside of the knowledge graph or an external entity of any type."@en ;
               rdfs:isDefinedBy eurio: ;
               rdfs:label "refers to"@en .


#################################################################
#    Data properties
#################################################################

###  http://data.europa.eu/s66#abstract
eurio:abstract rdf:type owl:DatatypeProperty ;
               rdfs:range xsd:string ;
               rdfs:comment "The general summary and ideas of a CORDIS entity, e.g., project, result."@en ;
               rdfs:isDefinedBy eurio: ;
               rdfs:label "abstract"@en .


###  http://data.europa.eu/s66#additionalName
eurio:additionalName rdf:type owl:DatatypeProperty ;
                     rdfs:domain eurio:Person ;
                     rdfs:range xsd:string ;
                     rdfs:comment "An additional name for a Person, can be used for a middle name."@en ;
                     rdfs:isDefinedBy eurio: ;
                     rdfs:label "additional name"@en .


###  http://data.europa.eu/s66#addressCountry
eurio:addressCountry rdf:type owl:DatatypeProperty ;
                     rdfs:domain eurio:PostalAddress ;
                     rdfs:range xsd:string ;
                     rdfs:comment "The country of the place or address. You can also provide the two-letter ISO 3166-1 alpha-2 country code."@en ;
                     rdfs:isDefinedBy eurio: ;
                     rdfs:label "address country"@en .


###  http://data.europa.eu/s66#addressLocality
eurio:addressLocality rdf:type owl:DatatypeProperty ;
                      rdfs:domain eurio:PostalAddress ;
                      rdfs:range xsd:string ;
                      rdfs:comment "The locality, town or city of the place or address."@en ;
                      rdfs:isDefinedBy eurio: ;
                      rdfs:label "address locality"@en .


###  http://data.europa.eu/s66#authorList
eurio:authorList rdf:type owl:DatatypeProperty ;
                 rdfs:range xsd:string ;
                 rdfs:comment "The list of authors."@en ;
                 rdfs:isDefinedBy eurio: ;
                 rdfs:label "author list"@en .


###  http://data.europa.eu/s66#citationsNumber
#eurio:citationsNumber rdf:type owl:DatatypeProperty ;
#                      rdfs:domain eurio:Result ;
#                      rdfs:range xsd:nonNegativeInteger ;
#                      rdfs:comment "The number of citations of a published work."@en ;
#                      rdfs:isDefinedBy eurio: ;
#                      rdfs:label "citations number"@en .


###  http://data.europa.eu/s66#code
eurio:code rdf:type owl:DatatypeProperty ,
                    owl:FunctionalProperty ;
           rdfs:domain eurio:FundingScheme ;
           rdfs:range xsd:string ;
           rdfs:comment "A CORDA code."@en ;
           rdfs:isDefinedBy eurio: ;
           rdfs:label "code"@en .


###  http://data.europa.eu/s66#currency
eurio:currency rdf:type owl:DatatypeProperty ;
               rdfs:domain eurio:MonetaryAmount ;
               rdfs:range xsd:string ;
               rdfs:comment "The currency in which the monetary amount is expressed."@en ;
               rdfs:isDefinedBy eurio: ;
               rdfs:label "currency"@en .


###  http://data.europa.eu/s66#date
eurio:date rdf:type owl:DatatypeProperty ;
           rdfs:range xsd:date ;
           rdfs:comment "The date in which the grant payment took place."@en ;
           rdfs:isDefinedBy eurio: ;
           rdfs:label "date"@en .


###  http://data.europa.eu/s66#definition
eurio:definition rdf:type owl:DatatypeProperty ;
                 rdfs:domain eurio:Acronym ;
                 rdfs:range xsd:string ;
                 rdfs:comment "The definition of the acronym."@en ;
                 rdfs:isDefinedBy eurio: ;
                 rdfs:label "definition"@en .


###  http://data.europa.eu/s66#description
eurio:description rdf:type owl:DatatypeProperty ;
                  rdfs:range xsd:string ;
                  rdfs:comment "A brief summary of the entity (project, etc.)."@en ;
                  rdfs:isDefinedBy eurio: ;
                  rdfs:label "description"@en .


###  http://data.europa.eu/s66#doi
eurio:doi rdf:type owl:DatatypeProperty ,
                   owl:FunctionalProperty ;
          rdfs:range xsd:anyURI ;
          rdfs:comment "The digital object identifier of a publication."@en ;
          rdfs:isDefinedBy eurio: ;
          rdfs:label "doi"@en .


###  http://data.europa.eu/s66#duration
eurio:duration rdf:type owl:DatatypeProperty ;
               rdfs:range xsd:nonNegativeInteger ;
               rdfs:comment "The period of time an entity (e.g. project, grant, etc.) has taken, represented as number of months."@en ;
               rdfs:isDefinedBy eurio: ;
               rdfs:label "duration"@en .


###  http://data.europa.eu/s66#email
eurio:email rdf:type owl:DatatypeProperty ;
            rdfs:domain eurio:ContactPoint ;
            rdfs:range xsd:anyURI ;
            rdfs:comment "Email address."@en ;
            rdfs:isDefinedBy eurio: ;
            rdfs:label "email"@en .


###  http://data.europa.eu/s66#endDate
eurio:endDate rdf:type owl:DatatypeProperty ;
              rdfs:subPropertyOf eurio:date ;
              rdfs:range xsd:date ;
              rdfs:comment "The date on which an entity (e.g. project, grant, etc.) is finalized or ceases to exist."@en ;
              rdfs:isDefinedBy eurio: ;
              rdfs:label "end date"@en .


###  http://data.europa.eu/s66#familyName
eurio:familyName rdf:type owl:DatatypeProperty ;
                 rdfs:domain eurio:Person ;
                 rdfs:range xsd:string ;
                 rdfs:comment "The family name (last name) of the person."@en ;
                 rdfs:isDefinedBy eurio: ;
                 rdfs:label "family name"@en .


###  http://data.europa.eu/s66#faxNumber
eurio:faxNumber rdf:type owl:DatatypeProperty ;
                rdfs:domain eurio:ContactPoint ;
                rdfs:range rdfs:Literal ;
                rdfs:comment "The fax number."@en ;
                rdfs:isDefinedBy eurio: ;
                rdfs:label "fax number"@en .


###  http://data.europa.eu/s66#finalResults
eurio:finalResults rdf:type owl:DatatypeProperty ;
                   rdfs:domain eurio:ProjectReportSummary ;
                   rdfs:range xsd:string ;
                   rdfs:comment "A brief description of the project findings."@en ;
                   rdfs:isDefinedBy eurio: ;
                   rdfs:label "final results"@en .


###  http://data.europa.eu/s66#fullAddress
eurio:fullAddress rdf:type owl:DatatypeProperty ;
                  rdfs:domain eurio:PostalAddress ;
                  rdfs:range rdfs:Literal ;
                  rdfs:comment "The full address of a physical location of an entity."@en ;
                  rdfs:isDefinedBy eurio: ;
                  rdfs:label "full address"@en .


###  http://data.europa.eu/s66#givenName
eurio:givenName rdf:type owl:DatatypeProperty ;
                rdfs:domain eurio:Person ;
                rdfs:range xsd:string ;
                rdfs:comment "The given name (first name) of the person."@en ;
                rdfs:isDefinedBy eurio: ;
                rdfs:label "given name"@en .


###  http://data.europa.eu/s66#honorificTitle
eurio:honorificTitle rdf:type owl:DatatypeProperty ;
                     rdfs:domain eurio:Person ;
                     rdfs:range xsd:string ;
                     rdfs:comment "An honorific prefix preceding a Person's name such as Dr, Mrs, Mr."@en ;
                     rdfs:isDefinedBy eurio: ;
                     rdfs:label "honorific title"@en .


###  http://data.europa.eu/s66#identifier
eurio:identifier rdf:type owl:DatatypeProperty ,
                          owl:FunctionalProperty ;
                 rdfs:range rdfs:Literal ;
                 rdfs:comment "The internal CORDA identifier."@en ;
                 rdfs:isDefinedBy eurio: ;
                 rdfs:label "identifier"@en .


###  http://data.europa.eu/s66#isNet
eurio:isNet rdf:type owl:DatatypeProperty ;
            rdfs:domain eurio:MonetaryAmount ;
            rdfs:range xsd:boolean ;
            rdfs:comment "Represents whether the monetary amount has deducted taxes or not. "@en ;
            rdfs:isDefinedBy eurio: ;
            rdfs:label "is net"@en .


###  http://data.europa.eu/s66#isbn
eurio:isbn rdf:type owl:DatatypeProperty ,
                    owl:FunctionalProperty ;
           rdfs:domain eurio:ProjectPublication ;
           rdfs:range rdfs:Literal ;
           rdfs:comment "The international standard book number of book publications."@en ;
           rdfs:isDefinedBy eurio: ;
           rdfs:label "isbn"@en .


###  http://data.europa.eu/s66#issn
eurio:issn rdf:type owl:DatatypeProperty ,
                    owl:FunctionalProperty ;
           rdfs:domain eurio:ProjectPublication ;
           rdfs:range rdfs:Literal ;
           rdfs:comment "The international standard serial number of journal publications."@en ;
           rdfs:isDefinedBy eurio: ;
           rdfs:label "issn"@en .


###  http://data.europa.eu/s66#journalNumber
eurio:journalNumber rdf:type owl:DatatypeProperty ;
                    rdfs:domain eurio:ProjectPublication ;
                    rdfs:range rdfs:Literal ;
                    rdfs:comment "The journal number of a published result."@en ;
                    rdfs:isDefinedBy eurio: ;
                    rdfs:label "journal number"@en .


###  http://data.europa.eu/s66#journalTitle
eurio:journalTitle rdf:type owl:DatatypeProperty ;
                   rdfs:domain eurio:ProjectPublication ;
                   rdfs:range xsd:string ;
                   rdfs:comment "The title of the journal of a published result."@en ;
                   rdfs:isDefinedBy eurio: ;
                   rdfs:label "journal title"@en .


###  http://data.europa.eu/s66#keyword
eurio:keyword rdf:type owl:DatatypeProperty ;
              rdfs:range xsd:string ;
              rdfs:comment "Word or words that represent the main idea of a referred entity (e.g., project. project result, etc.)"@en ;
              rdfs:isDefinedBy eurio: ;
              rdfs:label "keyword"@en .


###  http://data.europa.eu/s66#latitude
eurio:latitude rdf:type owl:DatatypeProperty ;
               rdfs:domain eurio:Coordinates ;
               rdfs:range xsd:decimal ;
               rdfs:comment "The latitude of a location. For example 37.42242 (WGS 84)."@en ;
               rdfs:isDefinedBy eurio: ;
               rdfs:label "latitude"@en .


###  http://data.europa.eu/s66#legalName
eurio:legalName rdf:type owl:DatatypeProperty ;
                rdfs:domain eurio:Organisation ;
                rdfs:range xsd:string ;
                rdfs:comment "The official name of the organization, e.g. the registered company name."@en ;
                rdfs:isDefinedBy eurio: ;
                rdfs:label "legal name"@en .


###  http://data.europa.eu/s66#longitude
eurio:longitude rdf:type owl:DatatypeProperty ;
                rdfs:domain eurio:Coordinates ;
                rdfs:range xsd:decimal ;
                rdfs:comment "The longitude of a location. For example -122.08585 (WGS 84)."@en ;
                rdfs:isDefinedBy eurio: ;
                rdfs:label "longitude"@en .


###  http://data.europa.eu/s66#maxTrl
#eurio:maxTrl rdf:type owl:DatatypeProperty ;
#             rdfs:subPropertyOf eurio:trl ;
#             rdfs:range xsd:nonNegativeInteger ;
#             rdfs:comment "The maximum technological readiness level of a project."@en ;
#             rdfs:isDefinedBy eurio: ;
#             rdfs:label "max TRL"@en .


###  http://data.europa.eu/s66#minTrl
#eurio:minTrl rdf:type owl:DatatypeProperty ;
#             rdfs:subPropertyOf eurio:trl ;
#             rdfs:range xsd:nonNegativeInteger ;
#             rdfs:comment "The minimum technological readiness level of a project."@en ;
#             rdfs:isDefinedBy eurio: ;
#             rdfs:label "min TRL"@en .


###  http://data.europa.eu/s66#name
eurio:name rdf:type owl:DatatypeProperty ;
           rdfs:range xsd:string ;
           rdfs:comment "The name of an entity"@en ;
           rdfs:isDefinedBy eurio: ;
           rdfs:label "name"@en .


###  http://data.europa.eu/s66#order
eurio:order rdf:type owl:DatatypeProperty ;
            rdfs:domain eurio:OrganisationRole ;
            rdfs:range xsd:nonNegativeInteger .


###  http://data.europa.eu/s66#periodNumber
eurio:periodNumber rdf:type owl:DatatypeProperty ;
                   rdfs:domain eurio:ProjectReportSummary ;
                   rdfs:range xsd:integer ;
                   rdfs:comment "The number of the reporting period."@en ;
                   rdfs:isDefinedBy eurio: ;
                   rdfs:label "period number"@en .


###  http://data.europa.eu/s66#personMonths
#eurio:personMonths rdf:type owl:DatatypeProperty ;
#                   rdfs:domain eurio:ProjectDivision ;
#                   rdfs:range xsd:nonNegativeInteger ;
#                   rdfs:comment "The effort needed to carry out work contained in the project division, estimated in person-months."@en ;
#                   rdfs:isDefinedBy eurio: ;
#                   rdfs:label "person months"@en .


###  http://data.europa.eu/s66#postOfficeBoxNumber
eurio:postOfficeBoxNumber rdf:type owl:DatatypeProperty ;
                          rdfs:domain eurio:PostalAddress ;
                          rdfs:range rdfs:Literal ;
                          rdfs:comment "The post office box number for PO box addresses."@en ;
                          rdfs:isDefinedBy eurio: ;
                          rdfs:label "post office box number"@en .


###  http://data.europa.eu/s66#postalCode
eurio:postalCode rdf:type owl:DatatypeProperty ;
                 rdfs:domain eurio:PostalAddress ;
                 rdfs:range rdfs:Literal ;
                 rdfs:comment "The postal code of the place or address."@en ;
                 rdfs:isDefinedBy eurio: ;
                 rdfs:label "postal code"@en .


###  http://data.europa.eu/s66#projectStatus
eurio:projectStatus rdf:type owl:DatatypeProperty ;
                    rdfs:domain eurio:Project ;
                    rdfs:range [ rdf:type  rdfs:Datatype ;
                                 owl:oneOf ( "CANCEL" "CLOSED" "ONGOING" "SIGNED" "TERMINATED" ) ] ;
                    rdfs:comment "The current status (signed, ongoing, terminated, etc.) of the project."@en ;
                    rdfs:isDefinedBy eurio: ;
                    rdfs:label "project status"@en .


###  http://data.europa.eu/s66#publishedPages
eurio:publishedPages rdf:type owl:DatatypeProperty ;
                     rdfs:domain eurio:ProjectPublication ;
                     rdfs:range rdfs:Literal ;
                     rdfs:comment "The pages of a published result."@en ;
                     rdfs:isDefinedBy eurio: ;
                     rdfs:label "published pages"@en .


###  http://data.europa.eu/s66#publishedYear
eurio:publishedYear rdf:type owl:DatatypeProperty ;
                    rdfs:domain eurio:ProjectPublication ;
                    rdfs:range xsd:nonNegativeInteger ;
                    rdfs:comment "The year of publication."@en ;
                    rdfs:isDefinedBy eurio: ;
                    rdfs:label "published year"@en .


###  http://data.europa.eu/s66#publisher
eurio:publisher rdf:type owl:DatatypeProperty ;
                rdfs:domain eurio:ProjectPublication ;
                rdfs:range xsd:string ;
                rdfs:comment "Represents the publishing body of a published result."@en ;
                rdfs:isDefinedBy eurio: ;
                rdfs:label "publisher"@en .


###  http://data.europa.eu/s66#rcn
eurio:rcn rdf:type owl:DatatypeProperty ,
                   owl:FunctionalProperty ;
          rdfs:range xsd:nonNegativeInteger ;
          rdfs:comment "Internal CORDIS identifier used for the identification of the domain entities (e.g., projects, project results, organisations, funding schemes, etc.). Stands for Resource Control Number."@en ;
          rdfs:isDefinedBy eurio: ;
          rdfs:label "rcn"@en .


###  http://data.europa.eu/s66#roleLabel
eurio:roleLabel rdf:type owl:DatatypeProperty ;
                rdfs:domain eurio:OrganisationRole ;
                rdfs:range [ rdf:type  rdfs:Datatype ;
                             owl:oneOf ( "coordinator" "international partner" "participant" "partner"
                                         "third party" ) ] ;
                rdfs:comment "Title for capturing the role of an organisation."@en ;
                rdfs:isDefinedBy eurio: ;
                rdfs:label "role label"@en .


###  http://data.europa.eu/s66#shortForm
eurio:shortForm rdf:type owl:DatatypeProperty ;
                rdfs:domain eurio:Acronym ;
                rdfs:range xsd:string ;
                rdfs:comment "The value of the acronym."@en ;
                rdfs:isDefinedBy eurio: ;
                rdfs:label "short form"@en .


###  http://data.europa.eu/s66#signatureDate
eurio:signatureDate rdf:type owl:DatatypeProperty ;
                    rdfs:subPropertyOf eurio:date ;
                    rdfs:domain eurio:Project ;
                    rdfs:range xsd:date ;
                    rdfs:comment "The day a grant agreement has been signed."@en ;
                    rdfs:isDefinedBy eurio: ;
                    rdfs:label "signature date"@en .


###  http://data.europa.eu/s66#startDate
eurio:startDate rdf:type owl:DatatypeProperty ;
                rdfs:subPropertyOf eurio:date ;
                rdfs:range xsd:date ;
                rdfs:comment "The time an entity (e.g. project, grant, etc.) is initialized or starts to take effect."@en ;
                rdfs:isDefinedBy eurio: ;
                rdfs:label "start date"@en .


###  http://data.europa.eu/s66#streetAddress
eurio:streetAddress rdf:type owl:DatatypeProperty ;
                    rdfs:domain eurio:PostalAddress ;
                    rdfs:range rdfs:Literal ;
                    rdfs:comment "The street name and number of the place or address."@en ;
                    rdfs:isDefinedBy eurio: ;
                    rdfs:label "street address"@en .


###  http://data.europa.eu/s66#telephoneNumber
eurio:telephoneNumber rdf:type owl:DatatypeProperty ;
                      rdfs:domain eurio:ContactPoint ;
                      rdfs:range rdfs:Literal ;
                      rdfs:comment "The telephone number."@en ;
                      rdfs:isDefinedBy eurio: ;
                      rdfs:label "telephone number"@en .


###  http://data.europa.eu/s66#terminationDate
eurio:terminationDate rdf:type owl:DatatypeProperty ;
                      rdfs:subPropertyOf eurio:date ;
                      rdfs:range xsd:date ;
                      rdfs:comment "The termination date of a project."@en ;
                      rdfs:isDefinedBy eurio: ;
                      rdfs:label "termination date"@en .


###  http://data.europa.eu/s66#title
eurio:title rdf:type owl:DatatypeProperty ;
            rdfs:range rdfs:Literal ;
            rdfs:comment "The entity’s (e.g. project, work package, etc.) official name or title."@en ;
            rdfs:isDefinedBy eurio: ;
            rdfs:label "title"@en .


###  http://data.europa.eu/s66#trl
#eurio:trl rdf:type owl:DatatypeProperty ;
#          rdfs:domain [ rdf:type owl:Class ;
#                        owl:unionOf ( eurio:FundingScheme
#                                      eurio:Project
#                                    )
#                      ] ;
#          rdfs:range xsd:nonNegativeInteger ,
#                     [ rdf:type rdfs:Datatype ;
#                       owl:oneOf [ rdf:type rdf:List ;
#                                   rdf:first 1 ;
#                                   rdf:rest [ rdf:type rdf:List ;
#                                              rdf:first 2 ;
#                                              rdf:rest [ rdf:type rdf:List ;
#                                                         rdf:first 3 ;
#                                                         rdf:rest [ rdf:type rdf:List ;
#                                                                    rdf:first 4 ;
#                                                                    rdf:rest [ rdf:type rdf:List ;
#                                                                               rdf:first 5 ;
#                                                                               rdf:rest [ rdf:type rdf:List ;
#                                                                                          rdf:first 6 ;
#                                                                                          rdf:rest [ rdf:type rdf:List ;
#                                                                                                     rdf:first 7 ;
#                                                                                                     rdf:rest [ rdf:type rdf:List ;
#                                                                                                                rdf:first 8 ;
#                                                                                                                rdf:rest [ rdf:type rdf:List ;
#                                                                                                                           rdf:first 9 ;
#                                                                                                                           rdf:rest rdf:nil
#                                                                                                                         ]
#                                                                                                              ]
#                                                                                                   ]
#                                                                                        ]
#                                                                             ]
#                                                                  ]
#                                                       ]
#                                            ]
#                                 ]
#                     ] ;
#          rdfs:comment "The technological readiness level associated with a funding scheme or a project."@en ;
#          rdfs:isDefinedBy eurio: ;
#          rdfs:label "TRL"@en .


###  http://data.europa.eu/s66#url
eurio:url rdf:type owl:DatatypeProperty ;
          rdfs:range xsd:anyURI ;
          rdfs:comment "A URL that links internet resources related to a CORDIS entity."@en ;
          rdfs:isDefinedBy eurio: ;
          rdfs:label "URL"@en .


###  http://data.europa.eu/s66#value
eurio:value rdf:type owl:DatatypeProperty ;
            rdfs:range xsd:decimal ;
            rdfs:comment "The value of amount being expressed."@en ;
            rdfs:isDefinedBy eurio: ;
            rdfs:label "value"@en .


###  http://data.europa.eu/s66#vatNumber
eurio:vatNumber rdf:type owl:DatatypeProperty ;
                rdfs:domain eurio:Organisation ;
                rdfs:range xsd:string ;
                rdfs:comment "The unique number that identifies a taxable organisation or non-taxable legal entity that is registered for VAT."@en ;
                rdfs:isDefinedBy eurio: ;
                rdfs:label "VAT number"@en .


###  http://data.europa.eu/s66#workPerformed
eurio:workPerformed rdf:type owl:DatatypeProperty ;
                    rdfs:domain eurio:ProjectReportSummary ;
                    rdfs:range xsd:string ;
                    rdfs:comment "A summary of the work carried out during the development of the project."@en ;
                    rdfs:isDefinedBy eurio: ;
                    rdfs:label "work performed"@en .


#################################################################
#    Classes
#################################################################

###  http://data.europa.eu/s66#Acronym
eurio:Acronym rdf:type owl:Class ;
              rdfs:subClassOf [ rdf:type owl:Restriction ;
                                owl:onProperty eurio:definition ;
                                owl:cardinality 1;
                       ] ,
              [ rdf:type owl:Restriction ;
                owl:onProperty eurio:shortForm ;
                owl:cardinality 1;
                       ] ;
              rdfs:comment "An abbreviation formed from the initial letters of other words and pronounced as a word. It can refer to any type of entities in the CORDIS conceptual framework, and may be stated explicitly or extracted automatically from text."@en ;
              rdfs:isDefinedBy eurio: ;
              rdfs:label "Acronym"@en .


###  http://data.europa.eu/s66#AdministrativeArea
eurio:AdministrativeArea rdf:type owl:Class ;
                         rdfs:subClassOf [ rdf:type owl:Restriction ;
                                           owl:onProperty eurio:name ;
                                           owl:cardinality 1
                                  ] ;
                         rdfs:comment "An administrative geographical area that is typically managed by a public body. It can be a country, a region, a municipality, a province, a sub-municipality area, etc."@en ;
                         rdfs:isDefinedBy eurio: ;
                         rdfs:label "Administrative Area"@en ;
                         skos:broadMatch <http://data.europa.eu/m8g/AdminUnit> ,
                         <http://schema.org/AdministrativeArea> .


###  http://data.europa.eu/s66#Book
eurio:Book rdf:type owl:Class ;
           rdfs:subClassOf eurio:ProjectPublication ;
           rdfs:comment "A non-serial document that is complete in one volume or a designated finite number of volumes. A book published by a publisher is usually identified by an International Standard Book Number (ISBN), and may be manifested as a physical printed publication on paper bound in a hard or soft cover, or in electronic format as an 'e-book'."@en ;
           rdfs:isDefinedBy eurio: ;
           rdfs:label "Book"@en ;
           skos:broadMatch <http://purl.org/spar/fabio/Book> .


###  http://data.europa.eu/s66#BookChapter
eurio:BookChapter rdf:type owl:Class ;
                  rdfs:subClassOf eurio:ProjectPublication ;
                  rdfs:comment "A defined chapter of a book, usually with a separate title or number."@en ;
                  rdfs:isDefinedBy eurio: ;
                  rdfs:label "Book Chapter"@en ;
                  skos:broadMatch <http://purl.org/spar/fabio/BookChapter> .


###  http://data.europa.eu/s66#ConferencePaper
eurio:ConferencePaper rdf:type owl:Class ;
                      rdfs:subClassOf eurio:ProjectPublication ;
                      rdfs:comment "A paper, typically the realization of a research paper reporting original research findings, usually published within a conference proceedings volume."@en ;
                      rdfs:isDefinedBy eurio: ;
                      rdfs:label "Conference Paper"@en ;
                      skos:broadMatch <http://purl.org/spar/fabio/ConferencePaper> .


###  http://data.europa.eu/s66#ContactPoint
eurio:ContactPoint rdf:type owl:Class ;
                   rdfs:subClassOf [ rdf:type owl:Restriction ;
                                     owl:onProperty eurio:faxNumber ;
                                     owl:allValuesFrom xsd:string
                            ] ,
                   [ rdf:type owl:Restriction ;
                     owl:onProperty eurio:telephoneNumber ;
                     owl:allValuesFrom xsd:string
                            ] ;
                   rdfs:comment "A contact point of an organisation or a person."@en ;
                   rdfs:isDefinedBy eurio: ;
                   rdfs:label "Contact Point"@en .


###  http://data.europa.eu/s66#Coordinates
eurio:Coordinates rdf:type owl:Class ;
                  rdfs:subClassOf [ rdf:type owl:Restriction ;
                                    owl:onProperty eurio:latitude ;
                                    owl:cardinality 1
                           ] ,
                  [ rdf:type owl:Restriction ;
                    owl:onProperty eurio:longitude ;
                    owl:cardinality 1
                           ] ;
                  rdfs:comment "The geo coordinates for a location of entities that participate in or form part of research projects."@en ;
                  rdfs:isDefinedBy eurio: ;
                  rdfs:label "Coordinates"@en ;
                  skos:broadMatch <http://www.w3.org/ns/locn#Geometry> ;
                  skos:closeMatch schema:GeoCoordinates .


###  http://data.europa.eu/s66#Country
eurio:Country rdf:type owl:Class ;
              rdfs:subClassOf eurio:AdministrativeArea ,
              [ rdf:type owl:Restriction ;
                owl:onProperty eurio:hasEUCountryCode ;
                owl:maxCardinality 1
                       ] ;
              rdfs:comment "A country"@en ;
              rdfs:isDefinedBy eurio: ;
              rdfs:label "Country"@en ;
              skos:broadMatch schema:Country .


###  http://data.europa.eu/s66#DetectedAcronym
eurio:DetectedAcronym rdf:type owl:Class ;
                      rdfs:subClassOf eurio:Acronym ;
                      owl:disjointWith eurio:TitleAcronym ;
                      rdfs:comment "Any acronym that has been detected, automatically or manually, from the description of an entity or from any other form of natural language text."@en ;
                      rdfs:isDefinedBy eurio: ;
                      rdfs:label "Detected Acronym"@en .


###  http://data.europa.eu/s66#Event
#eurio:Event rdf:type owl:Class ;
#            rdfs:subClassOf [ rdf:type owl:Restriction ;
#                              owl:onProperty eurio:title ;
#                              owl:allValuesFrom xsd:string
#                            ] ,
#                            [ rdf:type owl:Restriction ;
#                              owl:onProperty eurio:title ;
#                              owl:cardinality 1
#                            ] ,
#                            [ rdf:type owl:Restriction ;
#                              owl:onProperty eurio:endDate ;
#                              owl:cardinality 1
#                            ] ,
#                            [ rdf:type owl:Restriction ;
#                              owl:onProperty eurio:startDate ;
#                              owl:cardinality 1
#                            ] ;
#            rdfs:comment "An event happening at a certain time and location, such as a meeting, lecture, or conference. In CORDIS, it represents the events are organized as part of or are related to research projects."@en ;
#            rdfs:isDefinedBy eurio: ;
#            rdfs:label "Event"@en ;
#            skos:broadMatch schema:Event .


###  http://data.europa.eu/s66#ExploitableResult
eurio:ExploitableResult rdf:type owl:Class ;
                        rdfs:subClassOf eurio:Result ;
                        rdfs:comment "An exploitable project result, e.g., a patent."@en ;
                        rdfs:isDefinedBy eurio: ;
                        rdfs:label "Exploitable Result"@en ;
                        skos:broadMatch <http://purl.org/spar/fabio/PatentDocument> .


###  http://data.europa.eu/s66#ForProfitOrganisation
eurio:ForProfitOrganisation rdf:type owl:Class ;
                            rdfs:subClassOf eurio:Organisation ;
                            rdfs:comment "A for profit entity"@en ;
                            rdfs:isDefinedBy eurio: ;
                            rdfs:label "For Profit Organisation"@en ;
                            skos:broadMatch dg:ForProfitOrganisation .


###  http://data.europa.eu/s66#FundingAgency
eurio:FundingAgency rdf:type owl:Class ;
                    rdfs:subClassOf eurio:Organisation ;
                    rdfs:comment "An organisation that materially administrates funding schemes and disburses related grants. In the context of CORDIS, it represents the various European agencies responsible for funding research projects (e.g. ERC, EASME, REA, etc.)."@en ;
                    rdfs:isDefinedBy eurio: ;
                    rdfs:label "Funding Agency"@en ;
                    skos:broadMatch dg:FundingAgency .


###  http://data.europa.eu/s66#FundingScheme
eurio:FundingScheme rdf:type owl:Class ;
                    rdfs:subClassOf [ rdf:type owl:Restriction ;
                                      owl:onProperty eurio:hasFundingSchemeCategory ;
                                      owl:cardinality 1
                             ] ,
                    [ rdf:type owl:Restriction ;
                      owl:onProperty eurio:isImplementedBy ;
                      owl:cardinality 1
                             ] ,
                    [ rdf:type owl:Restriction ;
                      owl:onProperty eurio:url ;
                      owl:minCardinality 1
                             ] ,
                    [ rdf:type owl:Restriction ;
                      owl:onProperty eurio:duration ;
                      owl:allValuesFrom xsd:nonNegativeInteger
                             ] ,
                    [ rdf:type owl:Restriction ;
                      owl:onProperty eurio:title ;
                      owl:allValuesFrom xsd:string
                             ] ,
                    [ rdf:type owl:Restriction ;
                      owl:onProperty eurio:title ;
                      owl:cardinality 1
                             ] ;
                    rdfs:comment "Set of rules and conditions which forms the basis for public funding of European research. In CORDIS, they represent the different legal frameworks (e.g. FP6, FP7, H2020). They can also be used to represent the different calls inside each framework by using the recursive relation “partOfScheme”."@en ;
                    rdfs:isDefinedBy eurio: ;
                    rdfs:label "Funding Scheme"@en ;
                    skos:broadMatch dg:FundingScheme .


###  http://data.europa.eu/s66#Grant
eurio:Grant rdf:type owl:Class ;
            rdfs:subClassOf [ rdf:type owl:Restriction ;
                              owl:onProperty eurio:funds ;
                              owl:minCardinality 1
                     ] ,
            [ rdf:type owl:Restriction ;
              owl:onProperty eurio:hasBeneficiary ;
              owl:minCardinality 1
                     ] ,
            [ rdf:type owl:Restriction ;
              owl:onProperty eurio:hasFundingScheme ;
              owl:minCardinality 1
                     ] ,
            [ rdf:type owl:Restriction ;
              owl:onProperty eurio:hasPayment ;
              owl:minCardinality 1
                     ] ,
            [ rdf:type owl:Restriction ;
              owl:onProperty eurio:hasFundingAmount ;
              owl:cardinality 1
                     ] ,
            [ rdf:type owl:Restriction ;
              owl:onProperty eurio:isDisbursedBy ;
              owl:cardinality 1
                     ] ,
            [ rdf:type owl:Restriction ;
              owl:onProperty eurio:duration ;
              owl:someValuesFrom xsd:nonNegativeInteger
                     ] ,
            [ rdf:type owl:Restriction ;
              owl:onProperty eurio:endDate ;
              owl:cardinality 1
                     ] ,
            [ rdf:type owl:Restriction ;
              owl:onProperty eurio:identifier ;
              owl:cardinality "1"^^xsd:nonNegativeInteger
                     ] ,
            [ rdf:type owl:Restriction ;
              owl:onProperty eurio:startDate ;
              owl:cardinality 1
                     ] ;
            rdfs:comment "A disbursed fund paid to a recipient or beneficiary within the context of a funded research project. In the context of CORDIS, it represents a grant of a specific EU programme (e.g. an H2020 grant)."@en ;
            rdfs:isDefinedBy eurio: ;
            rdfs:label "Grant"@en ;
            skos:broadMatch dg:Grant .


###  http://data.europa.eu/s66#GrantPayment
eurio:GrantPayment rdf:type owl:Class ;
                   rdfs:subClassOf [ rdf:type owl:Restriction ;
                                     owl:onProperty eurio:hasPaymentAmount ;
                                     owl:cardinality 1
                            ] ;
                   rdfs:comment "A single payment to a recipient or beneficiary of a Grant within a research project."@en ;
                   rdfs:isDefinedBy eurio: ;
                   rdfs:label "Grant Payment"@en ;
                   skos:broadMatch dg:GrantPayment .


###  http://data.europa.eu/s66#HigherOrSecondaryEducation
eurio:HigherOrSecondaryEducation rdf:type owl:Class ;
                                 rdfs:subClassOf eurio:Organisation ;
                                 rdfs:comment "Institution that provides education."@en ;
                                 rdfs:isDefinedBy eurio: ;
                                 rdfs:label "Higher Or Secondary Education"@en ;
                                 skos:broadMatch schema:EducationalOrganization, dg:EducationOrganisation  .


###  http://data.europa.eu/s66#JournalPaper
eurio:JournalPaper rdf:type owl:Class ;
                   rdfs:subClassOf eurio:ProjectPublication ;
                   rdfs:comment "An article, typically the realization of a research paper reporting original research findings, published in a journal issue."@en ;
                   rdfs:isDefinedBy eurio: ;
                   rdfs:label "Journal Paper"@en ;
                   skos:broadMatch <http://purl.org/spar/fabio/JournalArticle> .


###  http://data.europa.eu/s66#MonetaryAmount
eurio:MonetaryAmount rdf:type owl:Class ;
                     rdfs:subClassOf [ rdf:type owl:Restriction ;
                                       owl:onProperty eurio:isNet ;
                                       owl:maxCardinality 1
                              ] ,
                     [ rdf:type owl:Restriction ;
                       owl:onProperty eurio:value ;
                       owl:cardinality 1
                              ] ;
                     rdfs:comment "A monetary value or range. This type can be used to describe an amount of money such as $50 USD, or a range as in describing a bank account being suitable for a balance between £1,000 and £1,000,000 GBP, or the value of a salary, etc."@en ;
                     rdfs:isDefinedBy eurio: ;
                     rdfs:label "Monetary Amount"@en ;
                     skos:broadMatch schema:MonetaryAmount .


###  http://data.europa.eu/s66#NonPeerReviewedPublication
eurio:NonPeerReviewedPublication rdf:type owl:Class ;
                                 rdfs:subClassOf eurio:ProjectPublication ;
                                 rdfs:comment "A work that hasn't undergone peer reviewing prior to its publication."@en ;
                                 rdfs:isDefinedBy eurio: ;
                                 rdfs:label "Non Peer-Reviewed Publication"@en .


###  http://data.europa.eu/s66#Organisation
eurio:Organisation rdf:type owl:Class ;
                   rdfs:subClassOf [ rdf:type owl:Restriction ;
                                     owl:onProperty eurio:hasRole ;
                                     owl:allValuesFrom eurio:OrganisationRole
                            ] ,
                   [ rdf:type owl:Restriction ;
                     owl:onProperty eurio:hasSite ;
                     owl:minCardinality 1
                            ] ,
                   [ rdf:type owl:Restriction ;
                     owl:onProperty eurio:url ;
                     owl:maxCardinality 1
                            ] ,
                   [ rdf:type owl:Restriction ;
                     owl:onProperty eurio:identifier ;
                     owl:cardinality "1"^^xsd:nonNegativeInteger
                            ] ,
                   [ rdf:type owl:Restriction ;
                     owl:onProperty eurio:legalName ;
                     owl:cardinality 1
                            ] ,
                   [ rdf:type owl:Restriction ;
                     owl:onProperty eurio:rcn ;
                     owl:cardinality 1
                            ] ,
                   [ rdf:type owl:Restriction ;
                     owl:onProperty eurio:vatNumber ;
                     owl:cardinality 1
                            ] ;
                   owl:disjointWith eurio:Person ;
                   rdfs:comment "Represents a group of people, with the same purpose, organized together into a community or other social, commercial or political structure that participate in CORDIS projects."@en ;
                   rdfs:isDefinedBy eurio: ;
                   rdfs:label "Organisation"@en ;
                   skos:broadMatch org:Organization ,
                   dg:Organisation .


###  http://data.europa.eu/s66#OrganisationRole
eurio:OrganisationRole rdf:type owl:Class ;
                       rdfs:subClassOf eurio:Role ,
                       [ rdf:type owl:Restriction ;
                         owl:onProperty eurio:isRoleOf ;
                         owl:allValuesFrom eurio:Organisation
                                ] ,
                       [ rdf:type owl:Restriction ;
                         owl:onProperty eurio:isRoleOf ;
                         owl:cardinality 1
                                ] ;
                       owl:disjointWith eurio:PersonRole ;
                       rdfs:comment "Function assumed by or ascribed to an organisation that takes part in a particular project. In CORDIs, it represents roles such as coordinator, partner, consortium member, etc."@en ;
                       rdfs:isDefinedBy eurio: ;
                       rdfs:label "Organisation Role"@en ;
                       skos:broadMatch dg:OrganisationRole .


###  http://data.europa.eu/s66#OrganisationUnit
eurio:OrganisationUnit rdf:type owl:Class ;
                       rdfs:comment "A department or unit which is part of some larger Organization and only has full recognition within the context of that Organization. In CORDIS, it represents for instance the different departments of a university that participate in a particular project."@en ;
                       rdfs:isDefinedBy eurio: ;
                       rdfs:label "Organisation Unit"@en ;
                       skos:broadMatch org:OrganizationalUnit .


###  http://data.europa.eu/s66#Person
eurio:Person rdf:type owl:Class ;
             rdfs:subClassOf [ rdf:type owl:Restriction ;
                               owl:onProperty eurio:hasRole ;
                               owl:allValuesFrom eurio:PersonRole
                      ] ,
             [ rdf:type owl:Restriction ;
               owl:onProperty eurio:additionalName ;
               owl:maxCardinality 1
                      ] ,
             [ rdf:type owl:Restriction ;
               owl:onProperty eurio:familyName ;
               owl:cardinality 1
                      ] ,
             [ rdf:type owl:Restriction ;
               owl:onProperty eurio:givenName ;
               owl:cardinality 1
                      ] ;
             owl:disjointWith eurio:PersonRole ;
             rdfs:comment "A physical person. In CORDIS, it represents the different people assuming roles in research projects (e.g. PhD students, PIs, administrative contacts, etc.)."@en ;
             rdfs:isDefinedBy eurio: ;
             rdfs:label "Person"@en ;
             skos:broadMatch schema:Person ,
             dg:Person ;
             skos:closeMatch <http://www.w3.org/ns/person#Person> .


###  http://data.europa.eu/s66#PersonRole
eurio:PersonRole rdf:type owl:Class ;
                 rdfs:subClassOf eurio:Role ,
                 [ rdf:type owl:Restriction ;
                   owl:onProperty eurio:isRoleOf ;
                   owl:allValuesFrom  eurio:Person
                          ] ,
                 [ rdf:type owl:Restriction ;
                   owl:onProperty eurio:isRoleOf ;
                   owl:cardinality 1
                          ] ,
                 [ rdf:type owl:Restriction ;
                   owl:onProperty eurio:isEmployedBy ;
                   owl:maxCardinality 1
                          ] ;
                 rdfs:comment "Function assumed by or ascribed to a person that takes part in a particular project. In CORDIS, it represents roles such as contact person, PI, etc."@en ;
                 rdfs:isDefinedBy eurio: ;
                 rdfs:label "Person Role"@en ;
                 skos:broadMatch dg:PersonRole .


###  http://data.europa.eu/s66#PostalAddress
eurio:PostalAddress rdf:type owl:Class ;
                    rdfs:subClassOf [ rdf:type owl:Restriction ;
                                      owl:onProperty eurio:addressCountry ;
                                      owl:cardinality 1
                             ] ,
                    [ rdf:type owl:Restriction ;
                      owl:onProperty eurio:addressLocality ;
                      owl:cardinality 1
                             ] ,
                    [ rdf:type owl:Restriction ;
                      owl:onProperty eurio:fullAddress ;
                      owl:allValuesFrom xsd:string
                             ] ,
                    [ rdf:type owl:Restriction ;
                      owl:onProperty eurio:fullAddress ;
                      owl:cardinality 1
                             ] ,
                    [ rdf:type owl:Restriction ;
                      owl:onProperty eurio:postalCode ;
                      owl:allValuesFrom xsd:string ;
                             ] ,
                    [ rdf:type owl:Restriction ;
                      owl:onProperty eurio:postalCode ;
                      owl:cardinality 1
                             ] ,
                    [ rdf:type owl:Restriction ;
                      owl:onProperty eurio:streetAddress ;
                      owl:allValuesFrom xsd:string ;
                             ] ,
                    [ rdf:type owl:Restriction ;
                      owl:onProperty eurio:streetAddress ;
                      owl:cardinality 1
                             ] ;
                    rdfs:comment "The postal address of entities that participate in or form part of research projects."@en ;
                    rdfs:isDefinedBy eurio: ;
                    rdfs:label "Postal Address"@en ;
                    skos:broadMatch schema:PostalAddress ,
                    <http://www.w3.org/ns/locn#Address> .


###  http://data.europa.eu/s66#Project
eurio:Project rdf:type owl:Class ;
              rdfs:subClassOf [ rdf:type owl:Restriction ;
                                owl:onProperty eurio:hasInvolvedParty ;
                                owl:minCardinality 1
                       ] ,
              [ rdf:type owl:Restriction ;
                owl:onProperty eurio:isFundedBy ;
                owl:minCardinality 1
                       ] ,
              [ rdf:type owl:Restriction ;
                owl:onProperty eurio:hasTotalCost ;
                owl:cardinality 1
                       ] ,
              [ rdf:type owl:Restriction ;
                owl:onProperty eurio:url ;
                owl:maxCardinality 1
                       ] ,
              [ rdf:type owl:Restriction ;
                owl:onProperty eurio:abstract ;
                owl:cardinality 1
                       ] ,
              [ rdf:type owl:Restriction ;
                owl:onProperty eurio:duration ;
                owl:cardinality 1
                       ] ,
              [ rdf:type owl:Restriction ;
                owl:onProperty eurio:endDate ;
                owl:cardinality 1
                       ] ,
              [ rdf:type owl:Restriction ;
                owl:onProperty eurio:identifier ;
                owl:cardinality "1"^^xsd:nonNegativeInteger
                       ] ,
              [ rdf:type owl:Restriction ;
                owl:onProperty eurio:projectStatus ;
                owl:cardinality 1
                       ] ,
              [ rdf:type owl:Restriction ;
                owl:onProperty eurio:rcn ;
                owl:cardinality 1
                       ] ,
              [ rdf:type owl:Restriction ;
                owl:onProperty eurio:signatureDate ;
                owl:cardinality 1
                       ] ,
              [ rdf:type owl:Restriction ;
                owl:onProperty eurio:startDate ;
                owl:cardinality 1
                       ] ,
              [ rdf:type owl:Restriction ;
                owl:onProperty eurio:title ;
                owl:allValuesFrom  xsd:string
                       ] ,
              [ rdf:type owl:Restriction ;
                owl:onProperty eurio:title ;
                owl:cardinality 1
                       ] ;
              #owl:disjointWith eurio:ProjectDivision ;
              rdfs:comment "A planned research work that has one or more objectives (divided or not into tasks) and is conducted by one or more organisations. In CORDIS, it represents a project funded by an EU programme."@en ;
              rdfs:isDefinedBy eurio: ;
              rdfs:label "Project"@en ;
              skos:broadMatch dg:Project .


###  http://data.europa.eu/s66#ProjectDeliverable
eurio:ProjectDeliverable rdf:type owl:Class ;
                         rdfs:subClassOf eurio:Result ,
                         [ rdf:type owl:Restriction ;
                           owl:onProperty eurio:hasResultType ;
                           owl:cardinality 1
                                  ] ,
                         [ rdf:type owl:Restriction ;
                           owl:onProperty eurio:description ;
                           owl:maxCardinality 1
                                  ] ;
                         rdfs:comment "A document referring to the results obtained during the development of a project."@en ;
                         rdfs:isDefinedBy eurio: ;
                         rdfs:label "Project Deliverable"@en ;
                         skos:broadMatch <http://purl.org/spar/fabio/ProjectReportDocument> .


###  http://data.europa.eu/s66#ProjectDivision
#eurio:ProjectDivision rdf:type owl:Class ;
#                      rdfs:subClassOf [ rdf:type owl:Restriction ;
#                                        owl:onProperty eurio:personMonths ;
#                                        owl:cardinality 1
#                                      ] ,
#                                      [ rdf:type owl:Restriction ;
#                                        owl:onProperty eurio:description ;
#                                        owl:cardinality 1
#                                      ] ,
#                                      [ rdf:type owl:Restriction ;
#                                        owl:onProperty eurio:endDate ;
#                                        owl:cardinality 1
#                                      ] ,
#                                      [ rdf:type owl:Restriction ;
#                                        owl:onProperty eurio:startDate ;
#                                        owl:cardinality 1
#                                      ] ,
#                                      [ rdf:type owl:Restriction ;
#                                        owl:onProperty eurio:title ;
#                                        owl:allValuesFrom xsd:string
#                                      ] ,
#                                      [ rdf:type owl:Restriction ;
#                                        owl:onProperty eurio:title ;
#                                        owl:cardinality 1
#                                      ] ;
#                      rdfs:comment "An abstract entity that represents a part of the work and activities that need to be carried out within a project. This entity can be specialized through different sub-entities to represent the different types of project divisions."@en ;
#                      rdfs:isDefinedBy eurio: ;
#                      rdfs:label "Project Division"@en .


###  http://data.europa.eu/s66#ProjectPublication
eurio:ProjectPublication rdf:type owl:Class ;
                         rdfs:subClassOf eurio:Result ,
                         [ rdf:type owl:Restriction ;
                           owl:onProperty eurio:authorList ;
                           owl:cardinality 1
                                  ] ,
                         [ rdf:type owl:Restriction ;
                           owl:onProperty eurio:journalNumber ;
                           owl:allValuesFrom xsd:string
                                  ] ,
                         [ rdf:type owl:Restriction ;
                           owl:onProperty eurio:journalNumber ;
                           owl:cardinality 1
                                  ] ,
                         [ rdf:type owl:Restriction ;
                           owl:onProperty eurio:journalTitle ;
                           owl:cardinality 1
                                  ] ,
                         [ rdf:type owl:Restriction ;
                           owl:onProperty eurio:publishedPages ;
                           owl:allValuesFrom xsd:string
                                  ] ,
                         [ rdf:type owl:Restriction ;
                           owl:onProperty eurio:publishedPages ;
                           owl:maxCardinality 1
                                  ] ,
                         [ rdf:type owl:Restriction ;
                           owl:onProperty eurio:publishedYear ;
                           owl:cardinality 1
                                  ] ,
                         [ rdf:type owl:Restriction ;
                           owl:onProperty eurio:publisher ;
                           owl:cardinality 1
                                  ] ;
                         rdfs:comment "A scientific publication (e.g., journal article, conference paper, thesis dissertation, book, etc.) that resulted from the project activities."@en ;
                         rdfs:isDefinedBy eurio: ;
                         rdfs:label "Project Publication"@en ;
                         skos:broadMatch <http://purl.org/spar/fabio/Expression>.


###  http://data.europa.eu/s66#ProjectReportSummary
eurio:ProjectReportSummary rdf:type owl:Class ;
                           rdfs:subClassOf eurio:Result ,
                           [ rdf:type owl:Restriction ;
                             owl:onProperty eurio:abstract ;
                             owl:cardinality 1
                                    ] ,
                           [ rdf:type owl:Restriction ;
                             owl:onProperty eurio:endDate ;
                             owl:maxCardinality 1
                                    ] ,
                           [ rdf:type owl:Restriction ;
                             owl:onProperty eurio:finalResults ;
                             owl:maxCardinality 1
                                    ] ,
                           [ rdf:type owl:Restriction ;
                             owl:onProperty eurio:startDate ;
                             owl:maxCardinality 1
                                    ] ,
                           [ rdf:type owl:Restriction ;
                             owl:onProperty eurio:workPerformed ;
                             owl:maxCardinality 1
                                    ] ;
                           rdfs:comment "A document reporting on the progress of an on-going or completed project at a given period.."@en ;
                           rdfs:isDefinedBy eurio: ;
                           rdfs:label "Project Report Summary"@en ;
                           skos:broadMatch <http://purl.org/spar/fabio/ProjectReportSummary> .


###  http://data.europa.eu/s66#PublicBody
eurio:PublicBody rdf:type owl:Class ;
                 rdfs:subClassOf eurio:Organisation ;
                 rdfs:comment "Organisation or agency depending on a government, State or other supranational organisation and mainly operated by the government."@en ;
                 rdfs:isDefinedBy eurio: ;
                 rdfs:label "Public Body"@en ;
                 skos:closeMatch frapo:NotForProfitOrganization ,
                 dg:GovernamentalOrganisation .


###  http://data.europa.eu/s66#ResearchOrganisation
eurio:ResearchOrganisation rdf:type owl:Class ;
                           rdfs:subClassOf eurio:Organisation ;
                           rdfs:comment "Organisations devoted to research activities."@en ;
                           rdfs:isDefinedBy eurio: ;
                           rdfs:label "Research Organisation"@en ;
                           skos:broadMatch dg:ResearchPerformingOrganisation .


###  http://data.europa.eu/s66#Result
eurio:Result rdf:type owl:Class ;
             rdfs:subClassOf [ rdf:type owl:Restriction ;
                               owl:onProperty eurio:url ;
                               owl:maxCardinality 1
                      ] ,
             [ rdf:type owl:Restriction ;
               owl:onProperty eurio:title ;
               owl:allValuesFrom xsd:string
                      ] ,
             [ rdf:type owl:Restriction ;
               owl:onProperty eurio:title ;
               owl:cardinality 1 ;
                      ] ;
             rdfs:comment "Any tangible or intangible output of the project (such as data, knowledge and information, whatever their form or nature, whether or not they can be protected), which are generated in the project."@en ;
             rdfs:isDefinedBy eurio: ;
             rdfs:label "Result"@en .


###  http://data.europa.eu/s66#Role
eurio:Role rdf:type owl:Class ;
           rdfs:subClassOf [ rdf:type owl:Restriction ;
                             owl:onProperty eurio:isInvolvedIn ;
                             owl:cardinality 1
                    ] ,
           [ rdf:type owl:Restriction ;
             owl:onProperty eurio:endDate ;
             owl:cardinality 1
                    ] ,
           [ rdf:type owl:Restriction ;
             owl:onProperty eurio:roleLabel ;
             owl:cardinality 1
                    ] ,
           [ rdf:type owl:Restriction ;
             owl:onProperty eurio:startDate ;
             owl:cardinality 1
                    ] ;
           rdfs:comment "The function assumed by or ascribed to an entity (typically a person or organisation) in a particular project. It can be used to precise or represent additional information about a relationship or property such as participation or membership. In CORDIS, it represents the participation of a person or organisation in a research project."@en ;
           rdfs:isDefinedBy eurio: ;
           rdfs:label "Role"@en ;
           skos:broadMatch dg:Role .


###  http://data.europa.eu/s66#SME
eurio:SME rdf:type owl:Class ;
          rdfs:subClassOf eurio:Organisation ;
          rdfs:comment "Small and Medium Enterprises."@en ;
          rdfs:isDefinedBy eurio: ;
          rdfs:label "SME"@en ;
          skos:broadMatch frapo:SME .


###  http://data.europa.eu/s66#Site
eurio:Site rdf:type owl:Class ;
           rdfs:subClassOf [ rdf:type owl:Restriction ;
                             owl:onProperty eurio:hasGeographicalLocation ;
                             owl:minCardinality 1
                    ] ,
           [ rdf:type owl:Restriction ;
             owl:onProperty eurio:isSiteOf ;
             owl:cardinality 1
                    ] ,
           [ rdf:type owl:Restriction ;
             owl:onProperty eurio:hasAddress ;
             owl:cardinality 1
                    ] ,
           [ rdf:type owl:Restriction ;
             owl:onProperty eurio:hasCoordinates ;
             owl:cardinality 1
                    ] ,
           [ rdf:type owl:Restriction ;
             owl:onProperty eurio:name ;
             owl:cardinality 1
                    ] ;
           rdfs:comment "The physical extension of entities that participate in or form part of research projects."@en ;
           rdfs:isDefinedBy eurio: ;
           rdfs:label "Site"@en ;
           skos:broadMatch org:Site .


###  http://data.europa.eu/s66#Task
#eurio:Task rdf:type owl:Class ;
#           rdfs:subClassOf eurio:ProjectDivision ;
#           owl:disjointWith eurio:WorkPackage ;
#           rdfs:comment "A sub-division of a Work Package. Different tasks can proceed in parallel, within a work package, and cover one or more reporting periods of the project. A task must start and end with the time range of its parent Work Package."@en ;
#           rdfs:isDefinedBy eurio: ;
#           rdfs:label "Task"@en ;
#           skos:broadMatch oegp:Task .


###  http://data.europa.eu/s66#ThesisDissertation
eurio:ThesisDissertation rdf:type owl:Class ;
                         rdfs:subClassOf eurio:ProjectPublication ;
                         rdfs:comment "A book authored by a student containing a formal presentations of research outputs submitted for examination in completion of a course of study at an institution of higher education, to fulfil the requirements for an academic degree. Also know as a dissertation."@en ;
                         rdfs:isDefinedBy eurio: ;
                         rdfs:label "Thesis"@en ;
                         skos:broadMatch <http://purl.org/spar/fabio/Thesis> .


###  http://data.europa.eu/s66#TitleAcronym
eurio:TitleAcronym rdf:type owl:Class ;
                   rdfs:subClassOf eurio:Acronym ;
                   rdfs:comment "An acronym explicitly defined as the title or name of another entity (e.g. Project, Organisation, Funding Scheme, etc.)."@en ;
                   rdfs:isDefinedBy eurio: ;
                   rdfs:label "Title Acronym"@en .


###  http://data.europa.eu/s66#WorkPackage
#eurio:WorkPackage rdf:type owl:Class ;
#                  rdfs:subClassOf eurio:ProjectDivision ,
#                                  [ rdf:type owl:Restriction ;
#                                    owl:onProperty eurio:hasTask ;
#                                    owl:minCardinality 1
#                                  ] ;
#                  rdfs:comment "A major subdivision of a project which leads to the completion of one of the goals, objectives or major deliverables within the project. Different work packages can proceed in parallel within a project."@en ;
#                  rdfs:isDefinedBy eurio: ;
#                  rdfs:label "Work Package"@en ;
#                  skos:broadMatch oegp:WorkPackage .


###  http://data.europa.eu/s66#WorkshopPaper
eurio:WorkshopPaper rdf:type owl:Class ;
                    rdfs:subClassOf eurio:ProjectPublication ;
                    rdfs:comment "A paper, typically the realization of a research paper reporting original research findings, usually presented at a workshop and published within a workshop proceedings volume."@en ;
                    rdfs:isDefinedBy eurio: ;
                    rdfs:label "Workshop Paper"@en ;
                    skos:broadMatch <http://purl.org/spar/fabio/WorkshopPaper> .


###  http://www.w3.org/2004/02/skos/core#Concept
skos:Concept rdf:type owl:Class .


[ dcat:accessURL <http://data.europa.eu/s66#> ;
  dcat:downloadURL <http://data.europa.eu/s66#>
] .

[ foaf:mbox "cordis@publications.europa.eu"
 ] .

#################################################################
#    Annotations
#################################################################

dg:EducationOrganisation skos:broadMatch schema:EducationalOrganization .


#################################################################
#    General axioms
#################################################################

[ rdf:type owl:AllDisjointClasses ;
  owl:members ( eurio:ConferencePaper
                eurio:JournalPaper
                eurio:WorkshopPaper
              )
] .


[ rdf:type owl:AllDisjointClasses ;
  owl:members ( eurio:ExploitableResult
                eurio:ProjectDeliverable
                eurio:ProjectPublication
                eurio:ProjectReportSummary
              )
] .


[ rdf:type owl:AllDisjointClasses ;
  owl:members ( eurio:ForProfitOrganisation
                eurio:FundingAgency
                eurio:HigherOrSecondaryEducation
                eurio:PublicBody
                eurio:ResearchOrganisation
                eurio:SME
              )
] .


###  Generated by the OWL API (version 4.5.9.2019-02-01T07:24:44Z) https://github.com/owlcs/owlapi
